x86/Asmgenproof.v
@@ -372,12 +372,6 @@ Qed.
 - Mach register values and PPC register values agree.
 *)
 
-Inductive size_consisitency :  list (option Z) -> stackadt -> Prop :=
-  |size_consisitency_nil : size_consisitency nil nil
-  |size_consisitency_cons : forall lsz astack fr,
-      size_consisitency lsz astack ->
-      size_consisitency ((Some (frame_size_a fr))::lsz) ((fr::nil)::astack).
-
 Definition size_of_callstack (l: list stackframe): list (option Z) :=
   (fun x:stackframe =>
      match x with
@@ -387,6 +381,73 @@ Definition size_of_callstack (l: list stackframe): list (option Z) :=
           |_ => None
         end
      end) ## l.
+
+Inductive size_consistency :  list (option Z) -> stackadt -> Prop :=
+  |size_consistency_nil : size_consistency nil nil
+  |size_consistency_cons : forall lsz astack fr,
+      size_consistency lsz astack ->
+      size_consistency ((Some (frame_size_a fr))::lsz) ((fr::nil)::astack).
+
+Lemma sp_of_stack_pspnull : forall st fid idx,
+    sp_of_stack st = (fid::nil,idx::nil) -> parent_sp_stree st = Vnullptr.
+Proof.
+  intros. unfold parent_sp_stree. rewrite H. auto.
+Qed.
+
+Lemma append_nil_right : forall A (l:list A),
+    l++nil = l.
+Proof.
+  induction l. auto. simpl. congruence.
+Qed.
+
+Lemma sp_of_stack_pspsome : forall st f1 lf path idx2 idx1 id,
+    sp_of_stack st = (f1::(Some id)::lf, (path++(idx2::nil))++(idx1::nil)) ->
+    parent_sp_stree st = Vptr (Stack (Some id) (path++(idx2::nil)) 1%positive) Ptrofs.zero.
+Proof.
+  intros. unfold parent_sp_stree. rewrite H. simpl.
+  destruct path. auto. destruct path. auto. rewrite removelast_app. simpl.
+  rewrite append_nil_right. auto. congruence.
+Qed.
+
+Lemma sp_of_stack_return : forall st st' p' fid lf path idx,
+    return_stree st = Some (st',p') ->
+    sp_of_stack st = (fid::lf,path++(idx::nil)) ->
+    sp_of_stack st' = (lf,path).
+Proof.
+  induction st. intros. unfold sp_of_stack in *. destruct st. destruct o.
+  - simpl in *. destr_in H0. destruct p.
+    + admit.
+(*
+
+ destr_in H0. inv Heqp0. inv H0. simpl. destr_in H1. inv H1. destr_in Heqp.
+      inv Heqp.
+      exploit H; eauto. rewrite Heqp0.
+      destr_in H1. destr. inv Heqp.
+      destruct l2. simpl in *. inv H1.
+      assert (f::f0::l2 = (f::f0::nil)++l2). reflexivity. rewrite H0 in H1.
+      rewrite removelast_app in H1. simpl in H1. 
+      admit.
+      simpl. destr. intro.
+      simpl in *. destr. destr_in H1. destr_in Heqp1.
+      inv Heqp1. inv H1. *)
+    + destruct s. destruct o. simpl in *. inv H0.
+      repeat destr_in Heqo. inv H0. simpl in *. inv H1.
+      destruct path. simpl in H4. inv H4. auto. inv H4. destruct path; inv H2.
+  - simpl in H1. inv H1.
+Admitted.
+
+Definition sp_of_callstack (l:list stackframe) : list val :=
+  (fun x:stackframe =>
+     match x with
+       |Stackframe _ sp _ _ => sp
+     end) ## l.
+
+Inductive sp_consistency : (list fid * path) -> list val -> Prop :=
+  |sp_consistency_nil : sp_consistency (nil,nil) nil
+  |sp_consistency_cons : forall id sp lf path ls idx,
+      sp_consistency (lf,path) ls ->
+      sp = Vptr (Stack (Some id) (path++(idx::nil)) 1%positive) Ptrofs.zero ->
+      sp_consistency (((Some id)::lf),(path++(idx::nil))) (sp::ls).
 (*
 Inductive astack_consistency : Mach.state -> Prop :=
   |astack_consistency_state: forall fb tf m cs c rs sp
@@ -408,9 +469,10 @@ Inductive match_states: Mach.state -> Asm.state -> Prop :=
         (MEXT: Mem.extends m m')
         (AT: transl_code_at_pc ge (rs PC) fb f c ep tf tc)
         (AG: agree ms sp rs)
-        (SC: size_consisitency
+        (SC: size_consistency
                ((Some (aligned_fsz (Mach.fn_stacksize f)))::(size_of_callstack s))
                (Mem.astack(Mem.support m)))
+        (SPC: sp_consistency (sp_of_stack (Mem.stack (Mem.support m))) (sp:: sp_of_callstack s))
         (AXP: ep = true -> rs#RAX = parent_sp s),
       match_states (Mach.State s fb sp c ms m)
                    (Asm.State rs m')
@@ -419,7 +481,8 @@ Inductive match_states: Mach.state -> Asm.state -> Prop :=
         (STACKS: match_stack ge s)
         (MEXT: Mem.extends m m')
         (AG: agree ms (parent_sp s) rs)
-        (SC:size_consisitency (size_of_callstack s) (Mem.astack(Mem.support m)))
+        (SC: size_consistency (size_of_callstack s) (Mem.astack(Mem.support m)))
+        (SPC: sp_consistency (sp_of_stack (Mem.stack (Mem.support m))) (sp_of_callstack s))
         (FB: fb = Global id)
         (ATPC: rs PC = Vptr fb Ptrofs.zero)
         (ATLR: rs RA = parent_ra s),
@@ -430,7 +493,8 @@ Inductive match_states: Mach.state -> Asm.state -> Prop :=
         (STACKS: match_stack ge s)
         (MEXT: Mem.extends m m')
         (AG: agree ms (parent_sp s) rs)
-        (SC:size_consisitency (size_of_callstack s) (Mem.astack(Mem.support m)))
+        (SC: size_consistency (size_of_callstack s) (Mem.astack(Mem.support m)))
+        (SPC: sp_consistency (sp_of_stack (Mem.stack (Mem.support m))) (sp_of_callstack s))
         (ATPC: rs PC = parent_ra s),
       match_states (Mach.Returnstate s ms m)
                    (Asm.State rs m').
@@ -440,9 +504,10 @@ Lemma exec_straight_steps:
   match_stack ge s ->
   Mem.extends m2 m2' ->
   Genv.find_funct_ptr ge fb = Some (Internal f) ->
-  size_consisitency
+  size_consistency
     ((Some (aligned_fsz (Mach.fn_stacksize f)))::(size_of_callstack s))
     (Mem.astack(Mem.support m2)) ->
+  sp_consistency (sp_of_stack (Mem.stack (Mem.support m2))) (sp:: sp_of_callstack s) ->
   transl_code_at_pc ge (rs1 PC) fb f (i :: c) ep tf tc ->
   (forall k c (TR: transl_instr f i ep k = OK c),
    exists rs2,
@@ -453,8 +518,8 @@ Lemma exec_straight_steps:
   plus step tge (State rs1 m1') E0 st' /\
   match_states (Mach.State s fb sp c ms2 m2) st'.
 Proof.
-  intros. inversion H3. subst. monadInv H8.
-  exploit H4; eauto. intros [rs2 [A [B C]]].
+  intros. inversion H4. subst. monadInv H9.
+  exploit H5; eauto. intros [rs2 [A [B C]]].
   exists (State rs2 m2'); split.
   eapply exec_straight_exec; eauto.
   econstructor; eauto. eapply exec_straight_at; eauto.
@@ -465,9 +530,10 @@ Lemma exec_straight_steps_goto:
   match_stack ge s ->
   Mem.extends m2 m2' ->
   Genv.find_funct_ptr ge fb = Some (Internal f) ->
-  size_consisitency
+  size_consistency
     (Some (aligned_fsz (Mach.fn_stacksize f))::(size_of_callstack s))
     (Mem.astack(Mem.support m2)) ->
+  sp_consistency (sp_of_stack (Mem.stack (Mem.support m2))) (sp:: sp_of_callstack s) ->
   Mach.find_label lbl f.(Mach.fn_code) = Some c' ->
   transl_code_at_pc ge (rs1 PC) fb f (i :: c) ep tf tc ->
   it1_is_parent ep i = false ->
@@ -480,10 +546,10 @@ Lemma exec_straight_steps_goto:
   plus step tge (State rs1 m1') E0 st' /\
   match_states (Mach.State s fb sp c' ms2 m2) st'.
 Proof.
-  intros. inversion H4. subst. monadInv H10.
-  exploit H6; eauto. intros [jmp [k' [rs2 [A [B C]]]]].
-  generalize (functions_transl _ _ _ H8 H9); intro FN.
-  generalize (transf_function_no_overflow _ _ H9); intro NOOV.
+  intros. inversion H5. subst. monadInv H11.
+  exploit H7; eauto. intros [jmp [k' [rs2 [A [B C]]]]].
+  generalize (functions_transl _ _ _ H9 H10); intro FN.
+  generalize (transf_function_no_overflow _ _ H10); intro NOOV.
   exploit exec_straight_steps_2; eauto.
   intros [ofs' [PC2 CT2]].
   exploit find_label_goto_label; eauto.
@@ -545,6 +611,7 @@ Proof.
   assert (Val.lessdef (rs src) (rs0 (preg_of src))). eapply preg_val; eauto.
   exploit Mem.storev_extends; eauto. intros [m2' [A B]].
   left; eapply exec_straight_steps; eauto.
+  erewrite <- Mem.support_storev; eauto.
   erewrite <- Mem.support_storev; eauto.
   rewrite (sp_val _ _ _ AG) in A. intros. simpl in TR.
   exploit storeind_correct; eauto. intros [rs' [P Q]].
@@ -618,6 +685,7 @@ Opaque loadind.
   exploit Mem.storev_extends; eauto. intros [m2' [C D]].
   left; eapply exec_straight_steps; eauto.
   erewrite <- Mem.support_storev; eauto.
+  erewrite <- Mem.support_storev; eauto.
   intros. simpl in TR.
   exploit transl_store_correct; eauto. intros [rs2 [P Q]].
   exists rs2; split. eauto.
@@ -685,6 +753,13 @@ Opaque loadind.
   assert (CTF:check_topframe (Mach.fn_stacksize f) (Mem.astack (Mem.support m'0)) = true).
    unfold check_topframe. inv SC.   inv MEXT. rewrite <- mext_sup. rewrite <- H14.
    rewrite pred_dec_true; auto.
+  assert (CSP:(parent_sp_stree (Mem.stack (Mem.support m'0)) = (parent_sp s))).
+  inv SPC. inv H14.
+  destruct s. simpl. inv MEXT. rewrite <- mext_sup. simpl in H11.
+  eapply sp_of_stack_pspnull; eauto.
+  simpl in H17. inv H17.
+  destruct s. simpl. inv H16. simpl. inv H16. inv MEXT. rewrite <- mext_sup. simpl in H11.
+  eapply sp_of_stack_pspsome. rewrite <- H11. eauto.
   destruct ros as [rf|fid]; simpl in H; monadInv H9.
 + (* Indirect call *)
   assert (rs rf = Vptr (Global id) Ptrofs.zero).
@@ -699,7 +774,8 @@ Opaque loadind.
   eapply plus_left. eapply exec_step_internal. eauto.
   eapply functions_transl; eauto. eapply find_instr_tail; eauto.
   simpl. replace (chunk_of_type Tptr) with Mptr in * by (unfold Tptr, Mptr; destruct Archi.ptr64; auto).
-  rewrite C. rewrite A. rewrite <- (sp_val _ _ _ AG). rewrite CTF. rewrite E. eauto. rewrite G. rewrite J. eauto.
+  rewrite C. rewrite A. rewrite <- (sp_val _ _ _ AG). rewrite CTF. rewrite CSP. rewrite pred_dec_true.
+  rewrite E. eauto. rewrite G. rewrite J. eauto. eauto.
   apply star_one. eapply exec_step_internal.
   transitivity (Val.offset_ptr rs0#PC Ptrofs.one). auto.
   rewrite <- H. simpl. eauto.
@@ -709,6 +785,7 @@ Opaque loadind.
   apply agree_set_other; auto. apply agree_nextinstr. apply agree_set_other; auto.
   eapply agree_change_sp; eauto. eapply parent_sp_def; eauto.
   inv SC. rewrite <- SF in H15. rewrite ASR in H15. rewrite ASP in H15. inv H15. auto.
+  inv SPC. admit. (*sp_of_stack and return*)
   Simplifs. rewrite Pregmap.gso; auto.
   generalize (preg_of_not_SP rf). rewrite (ireg_of_eq _ _ EQ1). congruence.
 + (* Direct call *)
@@ -717,7 +794,8 @@ Opaque loadind.
   eapply plus_left. eapply exec_step_internal. eauto.
   eapply functions_transl; eauto. eapply find_instr_tail; eauto.
   simpl. replace (chunk_of_type Tptr) with Mptr in * by (unfold Tptr, Mptr; destruct Archi.ptr64; auto).
-  rewrite C. rewrite A. rewrite <- (sp_val _ _ _ AG). rewrite CTF. rewrite E. eauto. rewrite G. rewrite J. eauto.
+  rewrite C. rewrite A. rewrite <- (sp_val _ _ _ AG). rewrite CTF. rewrite pred_dec_true.
+  rewrite E. eauto. rewrite G. rewrite J. eauto. eauto.
   apply star_one. eapply exec_step_internal.
   transitivity (Val.offset_ptr rs0#PC Ptrofs.one). auto. rewrite <- H. simpl. eauto.
   eapply functions_transl; eauto. eapply find_instr_tail; eauto.
@@ -726,6 +804,7 @@ Opaque loadind.
   apply agree_set_other; auto. apply agree_nextinstr. apply agree_set_other; auto.
   eapply agree_change_sp; eauto. eapply parent_sp_def; eauto.
   inv SC. rewrite <- SF in H13. rewrite ASR in H13. rewrite ASP in H13. inv H13. auto.
+  inv SPC. admit.
   rewrite Pregmap.gss. unfold Genv.symbol_address. rewrite symbols_preserved.
   repeat destr_in H0. rewrite H11. auto.
 
@@ -755,6 +834,7 @@ Opaque loadind.
   apply agree_nextinstr_nf. eapply agree_set_res; auto.
   eapply agree_undef_regs; eauto. intros; apply undef_regs_other_2; auto.
   erewrite <- external_call_astack; eauto.
+  admit. (*sp_of_stack and ext stack*)
   congruence.
 
 - (* Mgoto *)
@@ -881,12 +961,17 @@ Transparent destroyed_by_jumptable.
   assert (CTF:check_topframe (Mach.fn_stacksize f) (Mem.astack (Mem.support m'0)) = true).
    unfold check_topframe. inv SC.   inv MEXT. rewrite <- mext_sup. rewrite <- H13.
    rewrite pred_dec_true; auto.
+  assert (CSP: parent_sp_stree (Mem.stack (Mem.support m'0)) = parent_sp s).
+  inv SPC. inv H13.
+  destruct s. simpl. inv MEXT. rewrite <- mext_sup. simpl in H10. admit. (*sp_of_stack with parent_sp*) inv H16.
+  destruct s. simpl. inv H15. simpl. inv H15. inv MEXT. rewrite <- mext_sup. simpl in H10. admit.
   monadInv H8.
   exploit code_tail_next_int; eauto. intro CT1.
   left; econstructor; split.
   eapply plus_left. eapply exec_step_internal. eauto.
   eapply functions_transl; eauto. eapply find_instr_tail; eauto.
-  simpl. rewrite C. rewrite A. rewrite <- (sp_val _ _ _ AG). rewrite CTF. rewrite E. eauto. rewrite G. rewrite J. eauto.
+  simpl. rewrite C. rewrite A. rewrite <- (sp_val _ _ _ AG). rewrite CTF. rewrite pred_dec_true.
+  rewrite E. eauto. rewrite G. rewrite J. eauto. eauto.
   apply star_one. eapply exec_step_internal.
   transitivity (Val.offset_ptr rs0#PC Ptrofs.one). auto. rewrite <- H5. simpl. eauto.
   eapply functions_transl; eauto. eapply find_instr_tail; eauto.
@@ -897,6 +982,7 @@ Transparent destroyed_by_jumptable.
   inv SC. erewrite <- Mem.support_free in H12; eauto.
   erewrite Mem.astack_return_frame in H12; eauto.
   apply Mem.astack_pop_stage in H4. destruct H4. rewrite H4 in H12. inv H12. auto.
+  inv SPC. admit.
 - (* internal function *)
   exploit functions_translated; eauto. intros [tf [A B]]. monadInv B.
   generalize EQ; intros EQ'. monadInv EQ'.
@@ -936,6 +1022,7 @@ Transparent destroyed_at_function_entry.
   assert (aligned_fsz (Mach.fn_stacksize f) = frame_size_a (mk_frame (Mach.fn_stacksize f))).
   simpl. auto. rewrite H2. constructor; auto. erewrite Mem.astack_alloc. 2: eauto.
   erewrite <- Mem.astack_alloc_frame; eauto.
+  admit.
   intros. Simplifs. eapply agree_sp; eauto.
 
 - (* external function *)
@@ -952,13 +1039,13 @@ Transparent destroyed_at_function_entry.
   unfold loc_external_result. apply agree_set_other; auto. apply agree_set_pair; auto.
   apply agree_undef_caller_save_regs; auto.
   erewrite <- external_call_astack; eauto.
-
+  admit.
 - (* return *)
   inv STACKS. simpl in *.
   right. split. lia. split. auto.
   econstructor; eauto. rewrite ATPC; eauto. rewrite H3 in SC.
   auto. congruence.
-Qed.
+Admitted.
 
 Lemma transf_initial_states:
   forall st1, Mach.initial_state prog st1 ->
@@ -977,6 +1064,7 @@ Proof.
   unfold Vnullptr; destruct Archi.ptr64; congruence.
   intros. rewrite Regmap.gi. auto.
   erewrite Genv.init_mem_astack; eauto. simpl. constructor.
+  erewrite Genv.init_mem_stack; eauto. simpl. constructor.
   apply Genv.genv_vars_eq in H1 as H1'. auto.
   unfold Genv.symbol_address.
   rewrite (match_program_main TRANSF).
